some work to question 2 and started question 3

Labb2/Sorting/sorting.dfy
@@ -20,7 +20,44 @@ ensures sorted(s)
 {
 }
 
+predicate p(a : seq<int>, b : seq<int>)
+{
+   multiset(a) == multiset(b)
+}
+
 predicate p2(a : seq<int>, b : seq<int>)
 {
     forall i :: 0 <= i < |a| ==> a[i] in b
+}
+
+method checkSeq(a : seq<int>, b : seq<int>) returns (b : bool)
+{
+  var bArr := array(b);
+  var i := 0;
+  while (i < |a|)
+  {
+    if(a[i] in bArr){
+      var j := i;
+        while (j <= |bArr|)
+        {
+          if (a[i] == bArr[j]){
+          b := b[..j-1] + b[j-1..];
+        } else {
+          j := j + 1;
+        }
+      }
+    }else {
+      return false;
+    }
+    i := i + 1;
+  }
+    return true;
+  }
+}
+
+function sort(a : array<int>)
+modifies this.a;
+requires a != null;
+ensures sorted2(), p2(old(a), a);
+{
 }
