Labb2/Tokeneer/tokeneer.dfy
@@ -1,0 +1,15 @@
+class Token{
+  var fp : int;
+  var cl : int;
+
+  //for clearance: 0 = Low, 1 = Medium and 2 = High
+  method Init(fingerPrint : int, clearance : int)
+  modifies this;
+  requires 0 <= clearance <= 2;
+  ensures fp == fingerPrint && cl == clearance;
+  {
+    fp := fingerPrint;
+    cl := clearance;
+  }
+
+}
